typeclass/compiler/parsing/typeclass_well_formed_checkScript.sml
@@ -1,0 +1,221 @@
+open HolKernel Parse boolLib bossLib dep_rewrite BasicProvers;
+open pairTheory optionTheory listTheory pred_setTheory;
+open finite_mapTheory alistTheory;
+open balanced_mapTheory mlmapTheory miscTheory;
+open cycle_detectionTheory typeclass_tcexpTheory
+typeclass_env_map_implTheory;
+
+val _ = new_theory "typeclass_well_formed_check";
+
+(* check if there is cyclic superclass relation *)
+Definition superAList_def:
+  superAList cl_map =
+    MAP (λ(k,v). (k, v.super)) $ toAscList cl_map
+End
+
+Definition check_cl_map_no_cycles_def:
+  check_cl_map_no_cycles cl_map =
+    ¬has_cycle (superAList cl_map)
+End
+
+Theorem fmap_to_alist_MAP_KEYS:
+  INJ f (FDOM m) UNIV ⇒
+  set (fmap_to_alist (MAP_KEYS f m)) =
+    set (MAP (λ(k,v). (f k,v)) $ fmap_to_alist m)
+Proof
+  Induct_on `m` >>
+  rw[] >>
+  `INJ f (FDOM m) UNIV`
+  by (
+    drule_then irule INJ_SUBSET >>
+    simp[]
+  ) >>
+  drule_then (fn t => simp[t]) MAP_KEYS_FUPDATE >>
+  fs[EXTENSION,LAMBDA_PROD,GSYM PFORALL_THM] >>
+  rpt gen_tac >>
+  simp[MEM_MAP,MEM_fmap_to_alist,
+    LAMBDA_PROD,GSYM PEXISTS_THM,FLOOKUP_UPDATE] >>
+  iff_tac
+  >- (
+    IF_CASES_TAC
+    >- (
+      rw[] >>
+      irule_at (Pos hd) EQ_REFL >>
+      simp[]) >>
+    rw[MEM_MAP] >>
+    pairarg_tac >>
+    fs[] >>
+    irule_at (Pos hd) EQ_REFL >>
+    fs[FDOM_FLOOKUP,FAPPLY_FUPDATE_THM] >>
+    IF_CASES_TAC >>
+    fs[FLOOKUP_DEF]) >>
+  fs[MEM_MAP,FAPPLY_FUPDATE_THM,LAMBDA_PROD,
+    GSYM PEXISTS_THM] >>
+  rw[]
+  >- (
+    IF_CASES_TAC >>
+    fs[INJ_DEF] >>
+    spose_not_then kall_tac >>
+    pop_assum mp_tac >>
+    simp[]) >>
+  irule_at (Pos hd) EQ_REFL >>
+  IF_CASES_TAC >>
+  fs[FLOOKUP_DEF]
+QED
+
+Triviality set_MAP_SINGLE_FST_EQ:
+  (∀x y. f x = f y ⇔ x = y) ∧
+  set (MAP f x) = set (MAP f y) ⇒
+  set x = set y
+Proof
+  simp[LIST_TO_SET_MAP] >>
+  metis_tac[IMAGE_11]
+QED
+
+Triviality set_MAP_key_EQ:
+  set (MAP (λ(k,v). ({k},v)) x) = set (MAP (λ(k,v). ({k},v)) y) ⇒
+  set x = set y
+Proof
+  qpat_abbrev_tac `f=(λ(k,v). ({k},v))` >>
+  strip_tac >>
+  drule_at_then (Pos last) irule set_MAP_SINGLE_FST_EQ >>
+  rw[Abbr`f`,EQ_IMP_THM] >>
+  ntac 2 (pairarg_tac >> fs[])
+QED
+
+Theorem mlmap_toAscList:
+  map_ok (m:('a,'b) map) ⇒
+  SORTED (λ(x,y) (x',y'). (cmp_of m) x x' = Less) (toAscList m) ∧
+  (set (toAscList m)) =
+    set (fmap_to_alist (
+      (to_fmap: ('a,'b) map -> ('a |-> 'b)) m))
+Proof
+  Cases_on `m` >>
+  simp[map_ok_def,toAscList_def,cmp_of_def] >>
+  strip_tac >>
+  drule_then assume_tac comparisonTheory.TotOrder_imp_good_cmp >>
+  drule_all balanced_mapTheory.toAscList_thm >>
+  rw[] >>
+  drule_then assume_tac to_fmap_thm >>
+  drule_then assume_tac TotOrd_key_set >>
+  fs[lift_key_def,GSYM LIST_TO_SET_MAP,MAP_KEYS_def] >>
+  irule set_MAP_key_EQ >>
+  qmatch_goalsub_abbrev_tac `MAP _ (fmap_to_alist m)` >>
+  `INJ (λx. {x}) (FDOM m) UNIV` by simp[INJ_DEF] >>
+  drule fmap_to_alist_MAP_KEYS >>
+  rw[]
+QED
+
+Triviality ALL_DISTINCT_superAList:
+  map_ok cl_map ⇒
+  ALL_DISTINCT (MAP FST $ superAList cl_map)
+Proof
+  rw[superAList_def,map_fst] >>
+  simp[mlmapTheory.MAP_FST_toAscList]
+QED
+
+Triviality super_reachable_EQ_TC_depends_on:
+  map_ok cl_map ∧
+  (∀c d. FLOOKUP (to_fmap cl_map) c = SOME d ⇒
+    set d.super ⊆ FDOM (to_fmap cl_map)) ⇒
+  super_reachable (to_class_map cl_map) =
+    TC_depends_on (superAList cl_map)
+Proof
+  rw[super_reachable_def,TC_depends_on_def] >>
+  AP_TERM_TAC >>
+  rw[FUN_EQ_THM,superAList_def,map_fst] >>
+  fs[to_class_map_def,FLOOKUP_FMAP_MAP2,FMAP_MAP2_THM,PULL_EXISTS] >>
+  drule_then strip_assume_tac mlmap_toAscList >>
+  gvs[ALOOKUP_MAP,PULL_EXISTS,EXTENSION] >>
+  rw[EQ_IMP_THM]
+  >- (
+    drule_then assume_tac $ cj 2 MAP_FST_toAscList >>
+    drule_then assume_tac ALOOKUP_ALL_DISTINCT_MEM >>
+    drule_then strip_assume_tac mlmap_toAscList >>
+    gvs[EXTENSION] >>
+    qpat_assum `∀v k. FLOOKUP _ _ = _ ⇒ ALOOKUP _ _ = _` $
+      drule_then $ irule_at (Pos hd) >>
+    drule_then assume_tac $ cj 3 MAP_FST_toAscList >>
+    fs[SUBSET_DEF] >>
+    metis_tac[]
+  ) >>
+  drule_then assume_tac ALOOKUP_MEM >>
+  drule_then assume_tac $ cj 2 mlmap_toAscList >>
+  fs[EXTENSION,SUBSET_DEF]
+QED
+
+Theorem check_cl_map_no_cycles_IMP_super_no_cycles:
+  map_ok cl_map ∧
+  (∀c d. FLOOKUP (to_fmap cl_map) c = SOME d ⇒
+    set d.super ⊆ FDOM (to_fmap cl_map)) ∧
+  check_cl_map_no_cycles cl_map ⇒
+  super_no_cycles $ to_class_map cl_map
+Proof
+  rw[super_no_cycles_def] >>
+  drule_all_then assume_tac
+    super_reachable_EQ_TC_depends_on >>
+  drule_then assume_tac ALL_DISTINCT_superAList >>
+  drule_then assume_tac has_cycle_correct >>
+  fs[check_cl_map_no_cycles_def]
+QED
+
+(*
+Definition check_cl_map_def:
+  check_cl_map cl_map =
+  (all (\cl cl_info.
+    EVERY (\c. lookup cl_map c ≠ NONE) cl_info.super ∧
+    all (\name impl. lookup cl_info.methodsig name ≠ NONE) cl_info.defaults ∧
+    EVERY (\names. EVERY (\name. lookup cl_info.methodsig name ≠ NONE) names)
+    cl_info.minImp
+    ) cl_map ∧
+  check_cl_map_no_cycles cl_map)
+End
+
+Definition EVERY_instance_def:
+  EVERY_instance f inst_map =
+    all (\cl_name l. EVERY (\(ty,instinfo). f cl_name ty instinfo) l) inst_map
+End
+
+Definition has_instance_def:
+  has_instance inst_map cstr ty cl =
+    case lookup inst_map cl of
+       | NONE => F
+       | SOME l => ARB l
+End
+
+(* check if every instance satisfy the class requirements *)
+Definition check_inst_map_sat_cl_req_def:
+  check_inst_map_sat_cl_req inst_map cl_map = EVERY_instance
+    (\cl_name ty instinfo.
+      (case lookup cl_map cl_name of
+      | NONE => F
+      | SOME cl_info =>
+        (* implemented minImpl *)
+        EXISTS (\names. EVERY (\name. lookup instinfo.impl name ≠ NONE) names) cl_info.minImp ∧
+        (* implemented every method without function definitions *)
+        EVERY (\name sig. lookup cl_info.defaults name ≠ NONE ∨ lookup instinfo.impl name ≠ NONE) cl_info.methodsig ∧
+        (* TODO: implemented super classes *)
+        EVERY (has_instance inst_map instinfo.cstr ty) cl_map.super
+      ) ∧
+      (* check if constraints is valid *)
+      EVERY (λ(cl,v). lookup cl_map cl ≠ NONE ∧
+        TypeVar v ≠ ty (* v must be a variable in ty,
+          so we only need to test there
+          size are not equal to show its size is smaller than ty *)
+        ) instinfo.cstr
+     ) inst_map
+End
+
+(* the constraints must be scoped if the parser does not produce an error *)
+Theorem inst_cstr_scoped_type_var:
+Proof
+QED
+
+(* inst_map produced after the parsing does not contain
+* type that are alpha equivalent *)
+Theorem inst_map_no_alpha_equiv:
+Proof
+QED
+*)
+
+val _ = export_theory();
